src/Init/Data/Iterators/Lemmas/Combinators/Monadic/FilterMap.lean
@@ -292,7 +292,7 @@ theorem IterM.InternalConsumers.toList_filterMap {α β γ: Type w} {m : Type w 
   · simp
 
 theorem IterM.toList_map_eq_toList_mapM {α β γ : Type w}
-    {m : Type w → Type w'} [Monad m] [MonadAttach m] [LawfulMonad m] [LawfulMonadAttach m]
+    {m : Type w → Type w'} [Monad m] [MonadAttach m] [LawfulMonad m] [WeaklyLawfulMonadAttach m]
     [Iterator α m β] [Finite α m] [IteratorCollect α m m] [LawfulIteratorCollect α m m]
     {f : β → γ} {it : IterM (α := α) m β} :
     (it.map f).toList = (it.mapM fun b => pure (f b)).toList := by
@@ -303,14 +303,24 @@ theorem IterM.toList_map_eq_toList_mapM {α β γ : Type w}
   · simp only [PlausibleIterStep.yield, bind_pure_comp, pure_bind, Shrink.inflate_deflate,
       bind_map_left]
     conv => rhs; rhs; ext a; rw [← pure_bind (x := a.val) (f := fun _ => _ <$> _)]
-    simp only [← bind_assoc, bind_pure_comp, LawfulMonadAttach.map_attach]
+    simp only [← bind_assoc, bind_pure_comp, WeaklyLawfulMonadAttach.map_attach]
     simp [ihy ‹_›]
   · simp [ihs ‹_›]
   · simp
 
+theorem foo [Monad m] [MonadAttach m] (x : m (Option α)) (f : (_ : _) → _ → m β) :
+    MonadAttach.pbind x f = MonadAttach.pbind x (fun a ha => if h : a.isSome then f (some (a.get h)) (by simpa using ha) else f none (by simp_all)) := by
+  intros
+  congr
+  ext
+  split <;> rename_i heq
+  · simp
+  · simp only [Bool.not_eq_true, Option.isSome_eq_false_iff, Option.isNone_iff_eq_none] at heq
+    simp_all
+
 theorem IterM.toList_mapM_eq_toList_filterMapM {α β γ : Type w}
     {m : Type w → Type w'} {n : Type w → Type w''}
-    [Monad m] [LawfulMonad m] [Monad n] [MonadAttach n] [LawfulMonad n] [LawfulMonadAttach n]
+    [Monad m] [LawfulMonad m] [Monad n] [MonadAttach n] [LawfulMonad n] [WeaklyLawfulMonadAttach n]
     [MonadLiftT m n][LawfulMonadLiftT m n]
     [Iterator α m β] [Finite α m] [IteratorCollect α m n] [LawfulIteratorCollect α m n]
     {f : β → n γ} {it : IterM (α := α) m β} :
@@ -320,21 +330,17 @@ theorem IterM.toList_mapM_eq_toList_filterMapM {α β γ : Type w}
   rw [toList_eq_match_step, toList_eq_match_step, step_mapM, step_filterMapM, bind_assoc, bind_assoc]
   apply bind_congr; intro step
   split
-  · rename_i out _ _
-    simp only [PlausibleIterStep.yield, bind_pure_comp, bind_map_left, Shrink.inflate_deflate,
-      PlausibleIterStep.skip, bind_assoc]
-    rw [LawfulMonadAttach.bind_attach_of_nonempty]
-    rw [show ∀ g : γ → n (List γ), f out >>= g = (some <$> f out) >>= (fun a => if ha : a.isSome then g (a.get ha) else Classical.ofNonempty) by simp]
-    rw (occs := [1]) [← LawfulMonadAttach.map_attach (x := some <$> f out)]
-    simp only [dite_eq_ite, bind_map_left]
-    apply bind_congr; rintro ⟨fx, hfx⟩
-    obtain ⟨a, ha, rfl⟩ := LawfulMonadAttach.canReturn_map_imp' hfx
-    simp [ha, ihy ‹_›]
+  · conv =>
+      rhs
+      simp only [bind_pure_comp, bind_assoc]
+      simp only [MonadAttach.attach_bind_eq_pbind]
+      rw [foo]
+    simp [MonadAttach.attach_bind_eq_pbind, WeaklyLawfulMonadAttach.pbind_eq_bind, ihy ‹_›]
   · simp [ihs ‹_›]
   · simp
 
 theorem IterM.toList_map_eq_toList_filterMapM {α β γ : Type w} {m : Type w → Type w'}
-    [Monad m] [MonadAttach m] [LawfulMonad m] [LawfulMonadAttach m]
+    [Monad m] [MonadAttach m] [LawfulMonad m] [WeaklyLawfulMonadAttach m]
     [Iterator α m β] [Finite α m] [IteratorCollect α m m] [LawfulIteratorCollect α m m]
     {f : β → γ} {it : IterM (α := α) m β} :
     (it.map f).toList = (it.filterMapM fun b => pure (some (f b))).toList := by
@@ -345,8 +351,8 @@ theorem IterM.toList_map_eq_toList_filterMapM {α β γ : Type w} {m : Type w �
 theorem IterM.toList_filterMapM_filterMapM {α β γ δ : Type w}
     {m : Type w → Type w'} {n : Type w → Type w''} {o : Type w → Type w'''}
     [Monad m] [LawfulMonad m]
-    [Monad n] [MonadAttach n] [LawfulMonad n] [LawfulMonadAttach n]
-    [Monad o] [MonadAttach o] [LawfulMonad o] [LawfulMonadAttach o]
+    [Monad n] [MonadAttach n] [LawfulMonad n] [WeaklyLawfulMonadAttach n]
+    [Monad o] [MonadAttach o] [LawfulMonad o] [WeaklyLawfulMonadAttach o]
     [MonadLiftT m n] [MonadLiftT n o] [LawfulMonadLiftT m n] [LawfulMonadLiftT n o]
     [Iterator α m β] [Finite α m] [IteratorCollect α m m] [LawfulIteratorCollect α m m]
     {f : β → n (Option γ)} {g : γ → o (Option δ)}
@@ -366,20 +372,18 @@ theorem IterM.toList_filterMapM_filterMapM {α β γ δ : Type w}
   apply bind_congr; intro step
   split
   · simp only [bind_assoc, liftM_bind]
-    have {ε τ : Type _} (x : o (Option ε)) (f : (a : Option ε) → MonadAttach.CanReturn x a → o τ) :
-        MonadAttach.pbind x f = MonadAttach.pbind x (fun a ha => if h : a.isSome then f (some (a.get h)) (by simp [ha]) else f none (by simp_all)) := by
-      congr; ext a
-      cases a <;> simp +contextual
-    conv => rhs; simp only [LawfulMonadAttach.attach_bind_eq_pbind]
-    conv => rhs; rw [this]
-    simp only [bind_pure_comp, pure_bind, Shrink.inflate_deflate, LawfulMonadAttach.pbind_eq_bind,
-      bind_assoc]
-    conv => rhs; rw [← LawfulMonadAttach.map_attach (x := f _), liftM_map, bind_map_left]
+    conv =>
+      rhs
+      simp only [MonadAttach.attach_bind_eq_pbind]
+      rw [foo]
+      simp only [bind_pure_comp, pure_bind, Shrink.inflate_deflate,
+        WeaklyLawfulMonadAttach.pbind_eq_bind, bind_assoc]
+      rw [← WeaklyLawfulMonadAttach.map_attach (x := f _), liftM_map, bind_map_left]
     apply bind_congr; intro fx
     split
     · simp [ihy ‹_›]
     · simp only [liftM_pure, pure_bind, bind_assoc, Shrink.inflate_deflate]
-      conv => rhs; rw [← LawfulMonadAttach.map_attach (x := g _), bind_map_left]
+      conv => rhs; rw [← WeaklyLawfulMonadAttach.map_attach (x := g _), bind_map_left]
       apply bind_congr; intro gx
       split <;> simp [ihy ‹_›]
   · simp [ihs ‹_›]
@@ -388,8 +392,8 @@ theorem IterM.toList_filterMapM_filterMapM {α β γ δ : Type w}
 @[simp]
 theorem IterM.toList_filterMapM_mapM {α β γ δ : Type w}
     {m : Type w → Type w'} {n : Type w → Type w''} {o : Type w → Type w'''}
-    [Monad m] [LawfulMonad m] [Monad n] [MonadAttach n] [LawfulMonad n] [LawfulMonadAttach n]
-    [Monad o] [MonadAttach o] [LawfulMonad o] [LawfulMonadAttach o]
+    [Monad m] [LawfulMonad m] [Monad n] [MonadAttach n] [LawfulMonad n] [WeaklyLawfulMonadAttach n]
+    [Monad o] [MonadAttach o] [LawfulMonad o] [WeaklyLawfulMonadAttach o]
     [MonadLiftT m n] [MonadLiftT n o] [LawfulMonadLiftT m n] [LawfulMonadLiftT n o]
     [Iterator α m β] [Finite α m]
     {f : β → n γ} {g : γ → o (Option δ)}
@@ -406,17 +410,16 @@ theorem IterM.toList_filterMapM_mapM {α β γ δ : Type w}
   apply bind_congr; intro step
   split
   · simp only [bind_assoc, liftM_bind]
-    conv => rhs; simp only [LawfulMonadAttach.attach_bind_eq_pbind]
-    have {ε τ : Type _} (x : o (Option ε)) (f : (a : Option ε) → MonadAttach.CanReturn x a → o τ) :
-        MonadAttach.pbind x f = MonadAttach.pbind x (fun a ha => if h : a.isSome then f (some (a.get h)) (by simp [ha]) else f none (by simp_all)) := by
-      congr; ext a
-      cases a <;> simp +contextual
-    conv => rhs; rw [this]
-    simp only [liftM_pure, bind_pure_comp, pure_bind, Shrink.inflate_deflate, bind_assoc,
-      LawfulMonadAttach.pbind_eq_bind]
-    conv => rhs; rw [← LawfulMonadAttach.map_attach (x := f _), liftM_map, bind_map_left]
+    conv =>
+      rhs
+      simp only [MonadAttach.attach_bind_eq_pbind]
+      rw [foo]
+      simp only [bind_pure_comp, pure_bind, Shrink.inflate_deflate,
+        WeaklyLawfulMonadAttach.pbind_eq_bind, bind_assoc]
+      rw [← WeaklyLawfulMonadAttach.map_attach (x := f _), liftM_map, bind_map_left]
     apply bind_congr; intro fx
-    conv => rhs; rw [← LawfulMonadAttach.map_attach (x := g _), bind_map_left]
+    conv => rhs; rw [← WeaklyLawfulMonadAttach.map_attach (x := g _), bind_map_left]
+    simp only [liftM_pure, bind_pure_comp, pure_bind, Shrink.inflate_deflate, bind_assoc]
     apply bind_congr; intro gx
     split <;> simp [ihy ‹_›]
   · simp [ihs ‹_›]
@@ -425,7 +428,7 @@ theorem IterM.toList_filterMapM_mapM {α β γ δ : Type w}
 @[simp]
 theorem IterM.toList_filterMapM_map {α β γ δ : Type w}
     {m : Type w → Type w'} {n : Type w → Type w''}
-    [Monad m] [LawfulMonad m] [Monad n] [MonadAttach n] [LawfulMonad n] [LawfulMonadAttach n]
+    [Monad m] [LawfulMonad m] [Monad n] [MonadAttach n] [LawfulMonad n] [WeaklyLawfulMonadAttach n]
     [MonadLiftT m n] [LawfulMonadLiftT m n]
     [Iterator α m β] [Finite α m]
     {f : β → γ} {g : γ → n (Option δ)}
@@ -447,8 +450,8 @@ theorem IterM.toList_filterMapM_map {α β γ δ : Type w}
 @[simp]
 theorem IterM.toList_mapM_filterMapM {α β γ δ : Type w}
     {m : Type w → Type w'} {n : Type w → Type w''} {o : Type w → Type w'''}
-    [Monad m] [LawfulMonad m] [Monad n] [MonadAttach n] [LawfulMonad n] [LawfulMonadAttach n]
-    [Monad o] [MonadAttach o] [LawfulMonad o] [LawfulMonadAttach o]
+    [Monad m] [LawfulMonad m] [Monad n] [MonadAttach n] [LawfulMonad n] [WeaklyLawfulMonadAttach n]
+    [Monad o] [MonadAttach o] [LawfulMonad o] [WeaklyLawfulMonadAttach o]
     [MonadLiftT m n] [MonadLiftT n o] [LawfulMonadLiftT m n] [LawfulMonadLiftT n o]
     [Iterator α m β] [Finite α m] [IteratorCollect α m m] [LawfulIteratorCollect α m m]
     {f : β → n (Option γ)} {g : γ → o δ}
@@ -464,8 +467,8 @@ theorem IterM.toList_mapM_filterMapM {α β γ δ : Type w}
 @[simp]
 theorem IterM.toList_mapM_mapM {α β γ δ : Type w}
     {m : Type w → Type w'} {n : Type w → Type w''} {o : Type w → Type w'''}
-    [Monad m] [LawfulMonad m] [Monad n] [MonadAttach n] [LawfulMonad n] [LawfulMonadAttach n]
-    [Monad o] [MonadAttach o] [LawfulMonad o] [LawfulMonadAttach o]
+    [Monad m] [LawfulMonad m] [Monad n] [MonadAttach n] [LawfulMonad n] [WeaklyLawfulMonadAttach n]
+    [Monad o] [MonadAttach o] [LawfulMonad o] [WeaklyLawfulMonadAttach o]
     [MonadLiftT m n] [MonadLiftT n o] [LawfulMonadLiftT m n] [LawfulMonadLiftT n o]
     [Iterator α m β] [Finite α m] [IteratorCollect α m o] [LawfulIteratorCollect α m o]
     {f : β → n γ} {g : γ → o δ}
@@ -479,7 +482,7 @@ theorem IterM.toList_mapM_mapM {α β γ δ : Type w}
 @[simp]
 theorem IterM.toList_mapM_map {α β γ δ : Type w}
     {m : Type w → Type w'} {n : Type w → Type w''}
-    [Monad m] [LawfulMonad m] [Monad n] [MonadAttach n] [LawfulMonad n] [LawfulMonadAttach n]
+    [Monad m] [LawfulMonad m] [Monad n] [MonadAttach n] [LawfulMonad n] [WeaklyLawfulMonadAttach n]
     [MonadLiftT m n] [LawfulMonadLiftT m n]
     [Iterator α m β] [Finite α m] [IteratorCollect α m n] [LawfulIteratorCollect α m n]
     {f : β → γ} {g : γ → n δ}
@@ -491,7 +494,7 @@ theorem IterM.toList_mapM_map {α β γ δ : Type w}
 @[simp]
 theorem IterM.toList_map_mapM {α β γ δ : Type w}
     {m : Type w → Type w'} {n : Type w → Type w''}
-    [Monad m] [LawfulMonad m] [Monad n] [MonadAttach n] [LawfulMonad n] [LawfulMonadAttach n]
+    [Monad m] [LawfulMonad m] [Monad n] [MonadAttach n] [LawfulMonad n] [WeaklyLawfulMonadAttach n]
     [MonadLiftT m n] [LawfulMonadLiftT m n]
     [Iterator α m β] [Finite α m] [IteratorCollect α m n] [LawfulIteratorCollect α m n]
     {f : β → n γ} {g : γ → δ}
@@ -565,7 +568,7 @@ end ToList
 section ToListRev
 
 theorem IterM.toListRev_map_eq_toListRev_mapM {α β γ : Type w}
-    {m : Type w → Type w'} [Monad m] [MonadAttach m] [LawfulMonad m] [LawfulMonadAttach m]
+    {m : Type w → Type w'} [Monad m] [MonadAttach m] [LawfulMonad m] [WeaklyLawfulMonadAttach m]
     [Iterator α m β] [Finite α m] [IteratorCollect α m m] [LawfulIteratorCollect α m m]
     {f : β → γ} {it : IterM (α := α) m β} :
     (it.map f).toListRev = (it.mapM fun b => pure (f b)).toListRev := by
@@ -573,7 +576,7 @@ theorem IterM.toListRev_map_eq_toListRev_mapM {α β γ : Type w}
 
 theorem IterM.toListRev_mapM_eq_toListRev_filterMapM {α β γ : Type w}
     {m : Type w → Type w'} {n : Type w → Type w''}
-    [Monad m] [LawfulMonad m] [Monad n] [MonadAttach n] [LawfulMonad n] [LawfulMonadAttach n]
+    [Monad m] [LawfulMonad m] [Monad n] [MonadAttach n] [LawfulMonad n] [WeaklyLawfulMonadAttach n]
     [MonadLiftT m n][LawfulMonadLiftT m n]
     [Iterator α m β] [Finite α m] [IteratorCollect α m n] [LawfulIteratorCollect α m n]
     {f : β → n γ} {it : IterM (α := α) m β} :
@@ -582,7 +585,7 @@ theorem IterM.toListRev_mapM_eq_toListRev_filterMapM {α β γ : Type w}
   simp [toListRev_eq, toList_mapM_eq_toList_filterMapM]
 
 theorem IterM.toListRev_map_eq_toListRev_filterMapM {α β γ : Type w}
-    {m : Type w → Type w'} [Monad m] [MonadAttach m] [LawfulMonad m] [LawfulMonadAttach m]
+    {m : Type w → Type w'} [Monad m] [MonadAttach m] [LawfulMonad m] [WeaklyLawfulMonadAttach m]
     [Iterator α m β] [Finite α m] [IteratorCollect α m m] [LawfulIteratorCollect α m m]
     {f : β → γ} {it : IterM (α := α) m β} :
     (it.map f).toListRev = (it.filterMapM fun b => pure (some (f b))).toListRev := by
@@ -611,8 +614,8 @@ theorem IterM.toListRev_filter {α β : Type w} {m : Type w → Type w'} [Monad 
 theorem IterM.toListRev_filterMapM_filterMapM {α β γ δ : Type w}
     {m : Type w → Type w'} {n : Type w → Type w''} {o : Type w → Type w'''}
     [Monad m] [LawfulMonad m]
-    [Monad n] [MonadAttach n] [LawfulMonad n] [LawfulMonadAttach n]
-    [Monad o] [MonadAttach o] [LawfulMonad o] [LawfulMonadAttach o]
+    [Monad n] [MonadAttach n] [LawfulMonad n] [WeaklyLawfulMonadAttach n]
+    [Monad o] [MonadAttach o] [LawfulMonad o] [WeaklyLawfulMonadAttach o]
     [MonadLiftT m n] [MonadLiftT n o] [LawfulMonadLiftT m n] [LawfulMonadLiftT n o]
     [Iterator α m β] [Finite α m] [IteratorCollect α m m] [LawfulIteratorCollect α m m]
     {f : β → n (Option γ)} {g : γ → o (Option δ)}
@@ -629,8 +632,8 @@ theorem IterM.toListRev_filterMapM_filterMapM {α β γ δ : Type w}
 theorem IterM.toListRev_filterMapM_mapM {α β γ δ : Type w}
     {m : Type w → Type w'} {n : Type w → Type w''} {o : Type w → Type w'''}
     [Monad m] [LawfulMonad m]
-    [Monad n] [MonadAttach n] [LawfulMonad n] [LawfulMonadAttach n]
-    [Monad o] [MonadAttach o] [LawfulMonad o] [LawfulMonadAttach o]
+    [Monad n] [MonadAttach n] [LawfulMonad n] [WeaklyLawfulMonadAttach n]
+    [Monad o] [MonadAttach o] [LawfulMonad o] [WeaklyLawfulMonadAttach o]
     [MonadLiftT m n] [MonadLiftT n o] [LawfulMonadLiftT m n] [LawfulMonadLiftT n o]
     [Iterator α m β] [Finite α m] [IteratorCollect α m m] [LawfulIteratorCollect α m m]
     {f : β → n γ} {g : γ → o (Option δ)}
@@ -643,7 +646,7 @@ theorem IterM.toListRev_filterMapM_mapM {α β γ δ : Type w}
 @[simp]
 theorem IterM.toListRev_filterMapM_map {α β γ δ : Type w}
     {m : Type w → Type w'} {n : Type w → Type w''}
-    [Monad m] [LawfulMonad m] [Monad n] [MonadAttach n] [LawfulMonad n] [LawfulMonadAttach n]
+    [Monad m] [LawfulMonad m] [Monad n] [MonadAttach n] [LawfulMonad n] [WeaklyLawfulMonadAttach n]
     [MonadLiftT m n] [LawfulMonadLiftT m n]
     [Iterator α m β] [Finite α m] [IteratorCollect α m m] [LawfulIteratorCollect α m m]
     {f : β → γ} {g : γ → n (Option δ)}
@@ -656,8 +659,8 @@ theorem IterM.toListRev_filterMapM_map {α β γ δ : Type w}
 theorem IterM.toListRev_mapM_filterMapM {α β γ δ : Type w}
     {m : Type w → Type w'} {n : Type w → Type w''} {o : Type w → Type w'''}
     [Monad m] [LawfulMonad m]
-    [Monad n] [MonadAttach n] [LawfulMonad n] [LawfulMonadAttach n]
-    [Monad o] [MonadAttach o] [LawfulMonad o] [LawfulMonadAttach o]
+    [Monad n] [MonadAttach n] [LawfulMonad n] [WeaklyLawfulMonadAttach n]
+    [Monad o] [MonadAttach o] [LawfulMonad o] [WeaklyLawfulMonadAttach o]
     [MonadLiftT m n] [MonadLiftT n o] [LawfulMonadLiftT m n] [LawfulMonadLiftT n o]
     [Iterator α m β] [Finite α m] [IteratorCollect α m m] [LawfulIteratorCollect α m m]
     {f : β → n (Option γ)} {g : γ → o δ}
@@ -673,8 +676,8 @@ theorem IterM.toListRev_mapM_filterMapM {α β γ δ : Type w}
 @[simp]
 theorem IterM.toListRev_mapM_mapM {α β γ δ : Type w}
     {m : Type w → Type w'} {n : Type w → Type w''} {o : Type w → Type w'''}
-    [Monad m] [LawfulMonad m] [Monad n] [MonadAttach n] [LawfulMonad n] [LawfulMonadAttach n]
-    [Monad o] [MonadAttach o] [LawfulMonad o] [LawfulMonadAttach o]
+    [Monad m] [LawfulMonad m] [Monad n] [MonadAttach n] [LawfulMonad n] [WeaklyLawfulMonadAttach n]
+    [Monad o] [MonadAttach o] [LawfulMonad o] [WeaklyLawfulMonadAttach o]
     [MonadLiftT m n] [MonadLiftT n o] [LawfulMonadLiftT m n] [LawfulMonadLiftT n o]
     [Iterator α m β] [Finite α m]
     {f : β → n γ} {g : γ → o δ}
@@ -688,7 +691,7 @@ theorem IterM.toListRev_mapM_mapM {α β γ δ : Type w}
 @[simp]
 theorem IterM.toListRev_mapM_map {α β γ δ : Type w}
     {m : Type w → Type w'} {n : Type w → Type w''}
-    [Monad m] [LawfulMonad m] [Monad n] [MonadAttach n] [LawfulMonad n] [LawfulMonadAttach n]
+    [Monad m] [LawfulMonad m] [Monad n] [MonadAttach n] [LawfulMonad n] [WeaklyLawfulMonadAttach n]
     [MonadLiftT m n] [LawfulMonadLiftT m n]
     [Iterator α m β] [Finite α m] {f : β → γ} {g : γ → n δ} {it : IterM (α := α) m β} :
     ((it.map f).mapM g).toListRev =
@@ -701,7 +704,7 @@ end ToListRev
 section ToArray
 
 theorem IterM.toArray_map_eq_toArray_mapM {α β γ : Type w}
-    {m : Type w → Type w'} [Monad m] [MonadAttach m] [LawfulMonad m] [LawfulMonadAttach m]
+    {m : Type w → Type w'} [Monad m] [MonadAttach m] [LawfulMonad m] [WeaklyLawfulMonadAttach m]
     [Iterator α m β] [Finite α m] [IteratorCollect α m m] [LawfulIteratorCollect α m m]
     {f : β → γ} {it : IterM (α := α) m β} :
     (it.map f).toArray = (it.mapM fun b => pure (f b)).toArray := by
@@ -710,7 +713,7 @@ theorem IterM.toArray_map_eq_toArray_mapM {α β γ : Type w}
 theorem IterM.toArray_mapM_eq_toArray_filterMapM {α β γ : Type w}
     {m : Type w → Type w'} {n : Type w → Type w''}
     [Monad m] [LawfulMonad m]
-    [Monad n] [MonadAttach n] [LawfulMonad n] [LawfulMonadAttach n]
+    [Monad n] [MonadAttach n] [LawfulMonad n] [WeaklyLawfulMonadAttach n]
     [MonadLiftT m n][LawfulMonadLiftT m n]
     [Iterator α m β] [Finite α m] [IteratorCollect α m n] [LawfulIteratorCollect α m n]
     {f : β → n γ} {it : IterM (α := α) m β} :
@@ -718,7 +721,7 @@ theorem IterM.toArray_mapM_eq_toArray_filterMapM {α β γ : Type w}
   simp [← toArray_toList, toList_mapM_eq_toList_filterMapM]
 
 theorem IterM.toArray_map_eq_toArray_filterMapM {α β γ : Type w}
-    {m : Type w → Type w'} [Monad m] [MonadAttach m] [LawfulMonad m] [LawfulMonadAttach m]
+    {m : Type w → Type w'} [Monad m] [MonadAttach m] [LawfulMonad m] [WeaklyLawfulMonadAttach m]
     [Iterator α m β] [Finite α m] [IteratorCollect α m m] [LawfulIteratorCollect α m m]
     {f : β → γ} {it : IterM (α := α) m β} :
     (it.map f).toArray = (it.filterMapM fun b => pure (some (f b))).toArray := by
@@ -747,8 +750,8 @@ theorem IterM.toArray_filter {α : Type w} {m : Type w → Type w'} [Monad m] [L
 theorem IterM.toArray_filterMapM_filterMapM {α β γ δ : Type w}
     {m : Type w → Type w'} {n : Type w → Type w''} {o : Type w → Type w'''}
     [Monad m] [LawfulMonad m]
-    [Monad n] [MonadAttach n] [LawfulMonad n] [LawfulMonadAttach n]
-    [Monad o] [MonadAttach o] [LawfulMonad o] [LawfulMonadAttach o]
+    [Monad n] [MonadAttach n] [LawfulMonad n] [WeaklyLawfulMonadAttach n]
+    [Monad o] [MonadAttach o] [LawfulMonad o] [WeaklyLawfulMonadAttach o]
     [MonadLiftT m n] [MonadLiftT n o] [LawfulMonadLiftT m n] [LawfulMonadLiftT n o]
     [Iterator α m β] [Finite α m] [IteratorCollect α m m] [LawfulIteratorCollect α m m]
     {f : β → n (Option γ)} {g : γ → o (Option δ)}
@@ -765,8 +768,8 @@ theorem IterM.toArray_filterMapM_filterMapM {α β γ δ : Type w}
 theorem IterM.toArray_filterMapM_mapM {α β γ δ : Type w}
     {m : Type w → Type w'} {n : Type w → Type w''} {o : Type w → Type w'''}
     [Monad m] [LawfulMonad m]
-    [Monad n] [MonadAttach n] [LawfulMonad n] [LawfulMonadAttach n]
-    [Monad o] [MonadAttach o] [LawfulMonad o] [LawfulMonadAttach o]
+    [Monad n] [MonadAttach n] [LawfulMonad n] [WeaklyLawfulMonadAttach n]
+    [Monad o] [MonadAttach o] [LawfulMonad o] [WeaklyLawfulMonadAttach o]
     [MonadLiftT m n] [MonadLiftT n o] [LawfulMonadLiftT m n] [LawfulMonadLiftT n o]
     [Iterator α m β] [Finite α m]
     {f : β → n γ} {g : γ → o (Option δ)}
@@ -779,7 +782,7 @@ theorem IterM.toArray_filterMapM_mapM {α β γ δ : Type w}
 @[simp]
 theorem IterM.toArray_filterMapM_map {α β γ δ : Type w}
     {m : Type w → Type w'} {n : Type w → Type w''}
-    [Monad m] [LawfulMonad m] [Monad n] [MonadAttach n] [LawfulMonad n] [LawfulMonadAttach n]
+    [Monad m] [LawfulMonad m] [Monad n] [MonadAttach n] [LawfulMonad n] [WeaklyLawfulMonadAttach n]
     [MonadLiftT m n] [LawfulMonadLiftT m n]
     [Iterator α m β] [Finite α m] [IteratorCollect α m m] [LawfulIteratorCollect α m m]
     {f : β → γ} {g : γ → n (Option δ)}
@@ -791,8 +794,8 @@ theorem IterM.toArray_filterMapM_map {α β γ δ : Type w}
 @[simp]
 theorem IterM.toArray_mapM_filterMapM {α β γ δ : Type w}
     {m : Type w → Type w'} {n : Type w → Type w''} {o : Type w → Type w'''}
-    [Monad m] [LawfulMonad m] [Monad n] [MonadAttach n] [LawfulMonad n] [LawfulMonadAttach n]
-    [Monad o] [MonadAttach o] [LawfulMonad o] [LawfulMonadAttach o]
+    [Monad m] [LawfulMonad m] [Monad n] [MonadAttach n] [LawfulMonad n] [WeaklyLawfulMonadAttach n]
+    [Monad o] [MonadAttach o] [LawfulMonad o] [WeaklyLawfulMonadAttach o]
     [MonadLiftT m n] [MonadLiftT n o] [LawfulMonadLiftT m n] [LawfulMonadLiftT n o]
     [Iterator α m β] [Finite α m] [IteratorCollect α m m] [LawfulIteratorCollect α m m]
     {f : β → n (Option γ)} {g : γ → o δ}
@@ -808,8 +811,8 @@ theorem IterM.toArray_mapM_filterMapM {α β γ δ : Type w}
 @[simp]
 theorem IterM.toArray_mapM_mapM {α β γ δ : Type w}
     {m : Type w → Type w'} {n : Type w → Type w''} {o : Type w → Type w'''}
-    [Monad m] [LawfulMonad m] [Monad n] [MonadAttach n] [LawfulMonad n] [LawfulMonadAttach n]
-    [Monad o] [MonadAttach o] [LawfulMonad o] [LawfulMonadAttach o]
+    [Monad m] [LawfulMonad m] [Monad n] [MonadAttach n] [LawfulMonad n] [WeaklyLawfulMonadAttach n]
+    [Monad o] [MonadAttach o] [LawfulMonad o] [WeaklyLawfulMonadAttach o]
     [MonadLiftT m n] [MonadLiftT n o] [LawfulMonadLiftT m n] [LawfulMonadLiftT n o]
     [Iterator α m β] [Finite α m] [IteratorCollect α m o] [LawfulIteratorCollect α m o]
     {f : β → n γ} {g : γ → o δ}
@@ -822,7 +825,7 @@ theorem IterM.toArray_mapM_mapM {α β γ δ : Type w}
 @[simp]
 theorem IterM.toArray_mapM_map {α β γ δ : Type w}
     {m : Type w → Type w'} {n : Type w → Type w''}
-    [Monad m] [LawfulMonad m] [Monad n] [MonadAttach n] [LawfulMonad n] [LawfulMonadAttach n]
+    [Monad m] [LawfulMonad m] [Monad n] [MonadAttach n] [LawfulMonad n] [WeaklyLawfulMonadAttach n]
     [MonadLiftT m n] [LawfulMonadLiftT m n]
     [Iterator α m β] [Finite α m] [IteratorCollect α m n] [LawfulIteratorCollect α m n]
     {f : β → γ} {g : γ → n δ}
@@ -834,7 +837,7 @@ theorem IterM.toArray_mapM_map {α β γ δ : Type w}
 @[simp]
 theorem IterM.toArray_map_mapM {α β γ δ : Type w}
     {m : Type w → Type w'} {n : Type w → Type w''}
-    [Monad m] [LawfulMonad m] [Monad n] [MonadAttach n] [LawfulMonad n] [LawfulMonadAttach n]
+    [Monad m] [LawfulMonad m] [Monad n] [MonadAttach n] [LawfulMonad n] [WeaklyLawfulMonadAttach n]
     [MonadLiftT m n] [LawfulMonadLiftT m n]
     [Iterator α m β] [Finite α m] [IteratorCollect α m n] [LawfulIteratorCollect α m n]
     {f : β → n γ} {g : γ → δ}
@@ -853,7 +856,7 @@ theorem IterM.foldM_filterMapM {α β γ δ : Type w}
     {m : Type w → Type w'} {n : Type w → Type w''} {o : Type w → Type w'''}
     [Iterator α m β] [Finite α m]
     [Monad m] [LawfulMonad m]
-    [Monad n] [MonadAttach n] [LawfulMonad n] [LawfulMonadAttach n]
+    [Monad n] [MonadAttach n] [LawfulMonad n] [WeaklyLawfulMonadAttach n]
     [Monad o] [LawfulMonad o]
     [IteratorLoop α m n] [IteratorLoop α m o]
     [LawfulIteratorLoop α m n] [LawfulIteratorLoop α m o]
@@ -870,7 +873,7 @@ theorem IterM.foldM_filterMapM {α β γ δ : Type w}
   apply bind_congr; intro step
   cases step.inflate using PlausibleIterStep.casesOn
   · simp only [PlausibleIterStep.skip, PlausibleIterStep.yield, liftM_bind, bind_assoc]
-    conv => rhs; rw [← LawfulMonadAttach.map_attach (x := f _), liftM_map, bind_map_left]
+    conv => rhs; rw [← WeaklyLawfulMonadAttach.map_attach (x := f _), liftM_map, bind_map_left]
     apply bind_congr; intro c?
     split <;> simp [ihy ‹_›]
   · simp [ihs ‹_›]
@@ -880,7 +883,7 @@ theorem IterM.foldM_mapM {α β γ δ : Type w}
     {m : Type w → Type w'} {n : Type w → Type w''} {o : Type w → Type w'''}
     [Iterator α m β] [Finite α m]
     [Monad m] [LawfulMonad m]
-    [Monad n] [MonadAttach n] [LawfulMonad n] [LawfulMonadAttach n]
+    [Monad n] [MonadAttach n] [LawfulMonad n] [WeaklyLawfulMonadAttach n]
     [Monad o] [LawfulMonad o]
     [IteratorLoop α m n] [IteratorLoop α m o]
     [LawfulIteratorLoop α m n] [LawfulIteratorLoop α m o]
@@ -895,7 +898,7 @@ theorem IterM.foldM_mapM {α β γ δ : Type w}
   apply bind_congr; intro step
   cases step.inflate using PlausibleIterStep.casesOn
   · simp only [bind_pure_comp, liftM_map, bind_map_left, Shrink.inflate_deflate, bind_assoc]
-    conv => rhs; rw [← LawfulMonadAttach.map_attach (x := f _)]
+    conv => rhs; rw [← WeaklyLawfulMonadAttach.map_attach (x := f _)]
     simp [ihy ‹_›]
   · simp [ihs ‹_›]
   · simp
@@ -938,7 +941,7 @@ theorem IterM.foldM_map {α β γ δ : Type w} {m : Type w → Type w'} {n : Typ
 theorem IterM.fold_filterMapM {α β γ δ : Type w} {m : Type w → Type w'} {n : Type w → Type w''}
     [Iterator α m β] [Finite α m]
     [Monad m] [LawfulMonad m]
-    [Monad n] [MonadAttach n] [LawfulMonad n] [LawfulMonadAttach n]
+    [Monad n] [MonadAttach n] [LawfulMonad n] [WeaklyLawfulMonadAttach n]
     [IteratorLoop α m m] [IteratorLoop α m n]
     [LawfulIteratorLoop α m m] [LawfulIteratorLoop α m n]
     [MonadLiftT m n] [LawfulMonadLiftT m n]
@@ -952,7 +955,7 @@ theorem IterM.fold_filterMapM {α β γ δ : Type w} {m : Type w → Type w'} {n
 theorem IterM.fold_mapM {α β γ δ : Type w} {m : Type w → Type w'} {n : Type w → Type w''}
     [Iterator α m β] [Finite α m]
     [Monad m] [LawfulMonad m]
-    [Monad n] [MonadAttach n] [LawfulMonad n] [LawfulMonadAttach n]
+    [Monad n] [MonadAttach n] [LawfulMonad n] [WeaklyLawfulMonadAttach n]
     [IteratorLoop α m m] [IteratorLoop α m n]
     [LawfulIteratorLoop α m m] [LawfulIteratorLoop α m n]
     [MonadLiftT m n] [LawfulMonadLiftT m n]
@@ -1006,7 +1009,7 @@ section AnyAll
 theorem IterM.anyM_filterMapM {α β β' : Type w} {m : Type w → Type w'} {n : Type w → Type w''}
     [Iterator α m β] [Finite α m] [MonadLiftT m n]
     [Monad m] [LawfulMonad m]
-    [Monad n] [MonadAttach n] [LawfulMonad n] [LawfulMonadAttach n]
+    [Monad n] [MonadAttach n] [LawfulMonad n] [WeaklyLawfulMonadAttach n]
     {it : IterM (α := α) m β} {f : β → n (Option β')} {p : β' → n (ULift Bool)} :
     (it.filterMapM f).anyM p = (it.mapM (pure (f := n))).anyM (fun x => do
       match ← f x with
@@ -1020,12 +1023,12 @@ theorem IterM.anyM_filterMapM {α β β' : Type w} {m : Type w → Type w'} {n :
     simp only [bind_assoc, pure_bind, Shrink.inflate_deflate]
     have {x : n (ULift Bool)} : x = MonadAttach.attach (pure out) >>= (fun _ => x) := by
       rw (occs := [1]) [show x = pure out >>= (fun _ => x) by simp]
-      conv => lhs; rw [← LawfulMonadAttach.map_attach (x := pure out)]
+      conv => lhs; rw [← WeaklyLawfulMonadAttach.map_attach (x := pure out)]
       simp
     refine Eq.trans this ?_
-    simp only [LawfulMonadAttach.bind_attach_of_nonempty (x := pure out), pure_bind]
+    simp only [WeaklyLawfulMonadAttach.bind_attach_of_nonempty (x := pure out), pure_bind]
     split; rotate_left; rfl
-    conv => rhs; rw [← LawfulMonadAttach.map_attach (x := f _), bind_map_left]
+    conv => rhs; rw [← WeaklyLawfulMonadAttach.map_attach (x := f _), bind_map_left]
     apply bind_congr; intro fx
     split
     · simp [ihy ‹_›]
@@ -1038,7 +1041,7 @@ theorem IterM.anyM_filterMapM {α β β' : Type w} {m : Type w → Type w'} {n :
 
 theorem IterM.anyM_mapM {α β β' : Type w} {m : Type w → Type w'} {n : Type w → Type w''}
     [Iterator α m β] [Finite α m] [MonadLiftT m n]
-    [Monad m] [LawfulMonad m] [Monad n] [MonadAttach n] [LawfulMonad n] [LawfulMonadAttach n]
+    [Monad m] [LawfulMonad m] [Monad n] [MonadAttach n] [LawfulMonad n] [WeaklyLawfulMonadAttach n]
     {it : IterM (α := α) m β} {f : β → n β'} {p : β' → n (ULift Bool)} :
     (it.mapM f).anyM p = (it.mapM (pure (f := n))).anyM (fun x => do p (← f x)) := by
   induction it using IterM.inductSteps with | step it ihy ihs
@@ -1049,12 +1052,12 @@ theorem IterM.anyM_mapM {α β β' : Type w} {m : Type w → Type w'} {n : Type 
     simp only [bind_assoc, pure_bind, Shrink.inflate_deflate]
     have {x : n (ULift Bool)} : x = MonadAttach.attach (pure out) >>= (fun _ => x) := by
       rw (occs := [1]) [show x = pure out >>= (fun _ => x) by simp]
-      conv => lhs; rw [← LawfulMonadAttach.map_attach (x := pure out)]
+      conv => lhs; rw [← WeaklyLawfulMonadAttach.map_attach (x := pure out)]
       simp
     refine Eq.trans this ?_
-    simp only [LawfulMonadAttach.bind_attach_of_nonempty (x := pure out), pure_bind]
+    simp only [WeaklyLawfulMonadAttach.bind_attach_of_nonempty (x := pure out), pure_bind]
     split; rotate_left; rfl
-    conv => rhs; rw [← LawfulMonadAttach.map_attach (x := f _), bind_map_left]
+    conv => rhs; rw [← WeaklyLawfulMonadAttach.map_attach (x := f _), bind_map_left]
     apply bind_congr; intro fx
     simp [ihy ‹_›]
   · simp only [PlausibleIterStep.skip, pure_bind, bind_assoc]
@@ -1063,7 +1066,7 @@ theorem IterM.anyM_mapM {α β β' : Type w} {m : Type w → Type w'} {n : Type 
 
 theorem IterM.anyM_filterM {α β : Type w} {m : Type w → Type w'} {n : Type w → Type w''}
     [Iterator α m β] [Finite α m] [MonadLiftT m n]
-    [Monad m] [LawfulMonad m] [Monad n] [MonadAttach n] [LawfulMonad n] [LawfulMonadAttach n]
+    [Monad m] [LawfulMonad m] [Monad n] [MonadAttach n] [LawfulMonad n] [WeaklyLawfulMonadAttach n]
     {it : IterM (α := α) m β} {f : β → n (ULift Bool)} {p : β → n (ULift Bool)} :
     (it.filterM f).anyM p = (it.mapM (pure (f := n))).anyM (fun x => do
         if (← f x).down then
@@ -1078,12 +1081,12 @@ theorem IterM.anyM_filterM {α β : Type w} {m : Type w → Type w'} {n : Type w
     simp only [bind_assoc, pure_bind, Shrink.inflate_deflate]
     have {x : n (ULift Bool)} : x = MonadAttach.attach (pure out) >>= (fun _ => x) := by
       rw (occs := [1]) [show x = pure out >>= (fun _ => x) by simp]
-      conv => lhs; rw [← LawfulMonadAttach.map_attach (x := pure out)]
+      conv => lhs; rw [← WeaklyLawfulMonadAttach.map_attach (x := pure out)]
       simp
     refine Eq.trans this ?_
-    simp only [LawfulMonadAttach.bind_attach_of_nonempty (x := pure out), pure_bind]
+    simp only [WeaklyLawfulMonadAttach.bind_attach_of_nonempty (x := pure out), pure_bind]
     split; rotate_left; rfl
-    conv => rhs; rw [← LawfulMonadAttach.map_attach (x := f _), bind_map_left]
+    conv => rhs; rw [← WeaklyLawfulMonadAttach.map_attach (x := f _), bind_map_left]
     apply bind_congr; intro fx
     split <;> simp [ihy ‹_›]
   · simp only [PlausibleIterStep.skip, pure_bind, bind_assoc]
@@ -1147,7 +1150,7 @@ theorem IterM.anyM_filter {α β : Type w} {m : Type w → Type w'}
 
 theorem IterM.any_filterMapM {α β β' : Type w} {m : Type w → Type w'} {n : Type w → Type w''}
     [Iterator α m β] [Finite α m] [MonadLiftT m n] [IteratorLoop α m m]
-    [Monad m] [LawfulMonad m] [Monad n] [MonadAttach n] [LawfulMonad n] [LawfulMonadAttach n]
+    [Monad m] [LawfulMonad m] [Monad n] [MonadAttach n] [LawfulMonad n] [WeaklyLawfulMonadAttach n]
     [LawfulMonadLiftT m n] [LawfulIteratorLoop α m m]
     {it : IterM (α := α) m β} {f : β → n (Option β')} {p : β' → Bool} :
     (it.filterMapM f).any p = (it.mapM (pure (f := n))).anyM (fun x => do
@@ -1158,7 +1161,7 @@ theorem IterM.any_filterMapM {α β β' : Type w} {m : Type w → Type w'} {n : 
 
 theorem IterM.any_mapM {α β β' : Type w} {m : Type w → Type w'} {n : Type w → Type w''}
     [Iterator α m β] [Finite α m] [MonadLiftT m n] [IteratorLoop α m m]
-    [Monad m] [LawfulMonad m] [Monad n] [MonadAttach n] [LawfulMonad n] [LawfulMonadAttach n]
+    [Monad m] [LawfulMonad m] [Monad n] [MonadAttach n] [LawfulMonad n] [WeaklyLawfulMonadAttach n]
     [LawfulMonadLiftT m n] [LawfulIteratorLoop α m m]
     {it : IterM (α := α) m β} {f : β → n β'} {p : β' → Bool} :
     (it.mapM f).any p = (it.mapM (pure (f := n))).anyM (fun x => (.up <| p ·) <$> (f x)) := by
@@ -1166,7 +1169,7 @@ theorem IterM.any_mapM {α β β' : Type w} {m : Type w → Type w'} {n : Type w
 
 theorem IterM.any_filterM {α β : Type w} {m : Type w → Type w'} {n : Type w → Type w''}
     [Iterator α m β] [Finite α m] [MonadLiftT m n] [IteratorLoop α m m]
-    [Monad m] [LawfulMonad m] [Monad n] [MonadAttach n] [LawfulMonad n] [LawfulMonadAttach n]
+    [Monad m] [LawfulMonad m] [Monad n] [MonadAttach n] [LawfulMonad n] [WeaklyLawfulMonadAttach n]
     [LawfulMonadLiftT m n] [LawfulIteratorLoop α m m]
     {it : IterM (α := α) m β} {f : β → n (ULift Bool)} {p : β → Bool} :
     (it.filterM f).any p = (it.mapM (pure (f := n))).anyM (fun x => do
@@ -1212,7 +1215,7 @@ theorem IterM.any_map {α β β' : Type w} {m : Type w → Type w'}
 
 theorem IterM.allM_filterMapM {α β β' : Type w} {m : Type w → Type w'} {n : Type w → Type w''}
     [Iterator α m β] [Finite α m] [MonadLiftT m n]
-    [Monad m] [LawfulMonad m] [Monad n] [MonadAttach n] [LawfulMonad n] [LawfulMonadAttach n]
+    [Monad m] [LawfulMonad m] [Monad n] [MonadAttach n] [LawfulMonad n] [WeaklyLawfulMonadAttach n]
     [LawfulMonadLiftT m n]
     {it : IterM (α := α) m β} {f : β → n (Option β')} {p : β' → n (ULift Bool)} :
     (it.filterMapM f).allM p = (it.mapM (pure (f := n))).allM (fun x => do
@@ -1227,14 +1230,14 @@ theorem IterM.allM_filterMapM {α β β' : Type w} {m : Type w → Type w'} {n :
 
 theorem IterM.allM_mapM {α β β' : Type w} {m : Type w → Type w'} {n : Type w → Type w''}
     [Iterator α m β] [Finite α m] [MonadLiftT m n]
-    [Monad m] [LawfulMonad m] [Monad n] [MonadAttach n] [LawfulMonad n] [LawfulMonadAttach n]
+    [Monad m] [LawfulMonad m] [Monad n] [MonadAttach n] [LawfulMonad n] [WeaklyLawfulMonadAttach n]
     [LawfulMonadLiftT m n] {it : IterM (α := α) m β} {f : β → n β'} {p : β' → n (ULift Bool)} :
     (it.mapM f).allM p = (it.mapM (pure (f := n))).allM (fun x => do p (← f x)) := by
   simp [allM_eq_not_anyM_not, anyM_mapM]
 
 theorem IterM.allM_filterM {α β : Type w} {m : Type w → Type w'} {n : Type w → Type w''}
     [Iterator α m β] [Finite α m] [MonadLiftT m n]
-    [Monad m] [LawfulMonad m] [Monad n] [MonadAttach n] [LawfulMonad n] [LawfulMonadAttach n]
+    [Monad m] [LawfulMonad m] [Monad n] [MonadAttach n] [LawfulMonad n] [WeaklyLawfulMonadAttach n]
     [LawfulMonadLiftT m n]
     {it : IterM (α := α) m β} {f : β → n (ULift Bool)} {p : β → n (ULift Bool)} :
     (it.filterM f).allM p = (it.mapM (pure (f := n))).allM (fun x => do
@@ -1281,7 +1284,7 @@ theorem IterM.allM_filter {α β : Type w} {m : Type w → Type w'}
 
 theorem IterM.all_filterMapM {α β β' : Type w} {m : Type w → Type w'} {n : Type w → Type w''}
     [Iterator α m β] [Finite α m] [MonadLiftT m n] [IteratorLoop α m m]
-    [Monad m] [LawfulMonad m] [Monad n] [MonadAttach n] [LawfulMonad n] [LawfulMonadAttach n]
+    [Monad m] [LawfulMonad m] [Monad n] [MonadAttach n] [LawfulMonad n] [WeaklyLawfulMonadAttach n]
     [LawfulMonadLiftT m n] [LawfulIteratorLoop α m m]
     {it : IterM (α := α) m β} {f : β → n (Option β')} {p : β' → Bool} :
     (it.filterMapM f).all p = (it.mapM (pure (f := n))).allM (fun x => do
@@ -1292,7 +1295,7 @@ theorem IterM.all_filterMapM {α β β' : Type w} {m : Type w → Type w'} {n : 
 
 theorem IterM.all_mapM {α β β' : Type w} {m : Type w → Type w'} {n : Type w → Type w''}
     [Iterator α m β] [Finite α m] [MonadLiftT m n] [IteratorLoop α m m]
-    [Monad m] [LawfulMonad m] [Monad n] [MonadAttach n] [LawfulMonad n] [LawfulMonadAttach n]
+    [Monad m] [LawfulMonad m] [Monad n] [MonadAttach n] [LawfulMonad n] [WeaklyLawfulMonadAttach n]
     [LawfulMonadLiftT m n] [LawfulIteratorLoop α m m]
     {it : IterM (α := α) m β} {f : β → n β'} {p : β' → Bool} :
     (it.mapM f).all p = (it.mapM (pure (f := n))).allM (fun x => (.up <| p ·) <$> (f x)) := by
@@ -1300,7 +1303,7 @@ theorem IterM.all_mapM {α β β' : Type w} {m : Type w → Type w'} {n : Type w
 
 theorem IterM.all_filterM {α β : Type w} {m : Type w → Type w'} {n : Type w → Type w''}
     [Iterator α m β] [Finite α m] [MonadLiftT m n] [IteratorLoop α m m]
-    [Monad m] [LawfulMonad m] [Monad n] [MonadAttach n] [LawfulMonad n] [LawfulMonadAttach n]
+    [Monad m] [LawfulMonad m] [Monad n] [MonadAttach n] [LawfulMonad n] [WeaklyLawfulMonadAttach n]
     [LawfulMonadLiftT m n] [LawfulIteratorLoop α m m]
     {it : IterM (α := α) m β} {f : β → n (ULift Bool)} {p : β → Bool} :
     (it.filterM f).all p = (it.mapM (pure (f := n))).allM (fun x => do
